theories/SimModSemL.v
@@ -161,6 +161,8 @@ End W.
 
 
 
+Class gnames := { gnames_contents :> gname -> Prop }.
+Coercion gnames_contents: gnames >-> Funclass.
 
 Section SIM.
 
@@ -174,6 +176,8 @@ Section SIM.
   Variable wf: W -> Prop.
   Variable le: relation W.
   Hypothesis le_PreOrder: PreOrder le.
+
+  Context `{ns: gnames}.
 
   Variant _sim_itree (sim_itree: forall (R_src R_tgt: Type) (RR: st_local -> st_local -> R_src -> R_tgt -> Prop), Ord.t -> st_local * itree Es R_src -> st_local * itree Es R_tgt -> Prop)
           {R_src R_tgt} (RR: st_local -> st_local -> R_src -> R_tgt -> Prop)
@@ -461,6 +465,23 @@ Section SIM.
     :
       _sim_itree sim_itree RR i0 ((mrs_src0, fr_src0), i_src)
                  ((mrs_tgt0, fr_tgt0), trigger (FGet) >>= k_tgt)
+  (* | sim_itree_hint *)
+  (*     i0 i1 mrs_src0 mrs_tgt0 fr_src0 fr_tgt0 *)
+  (*     fn varg k_src i_tgt *)
+  (*     (ORD: Ord.lt i1 i0) *)
+  (*     (K: forall (HINT: namespace fn), *)
+  (*         sim_itree _ _ RR i1 ((mrs_src0, fr_src0), (trigger PushFrame;;; r <- trigger (Call fn varg);; trigger PopFrame;;; tau;; k_src r)) ((mrs_tgt0, fr_tgt0), i_tgt)) *)
+  (*   : *)
+  (*     _sim_itree sim_itree RR i0 ((mrs_src0, fr_src0), (trigger PushFrame;;; r <- trigger (Call fn varg);; trigger PopFrame;;; tau;; k_src r)) *)
+  (*                ((mrs_tgt0, fr_tgt0), i_tgt) *)
+  | sim_itree_call_fail
+      i0 mrs_src0 mrs_tgt0 fr_src0 fr_tgt0
+      fn varg k_src i_tgt
+      (FAIL: ~ ns fn)
+    :
+      _sim_itree sim_itree RR i0 ((mrs_src0, fr_src0), (trigger PushFrame;;; r <- trigger (Call fn varg);;
+                                                        trigger PopFrame;;; tau;; k_src r))
+                 ((mrs_tgt0, fr_tgt0), i_tgt)
   .
 
   Program Definition sim_itree: _ -> relation _ :=
@@ -680,6 +701,10 @@ Section SIM.
     + rewrite ! bind_bind. econs; eauto.
       { eapply OrdArith.lt_add_r; eauto. }
       eapply rclo6_clo_base. econs; eauto.
+    + erewrite f_equal2; [eapply sim_itree_call_fail| |]; cycle 1.
+      { f_equal. instantiate (3:=k_src0 >=> k_src). grind. }
+      { ss. }
+      { auto. }
   Qed.
 
   Lemma lbindC_spec: lbindC <7= gupaco6 (_sim_itree) (cpn6 (_sim_itree)).
@@ -802,11 +827,11 @@ Proof.
     exists mr0, mp. rewrite alist_add_find_neq; auto.
 Qed.
 
-Lemma self_sim_itree `{Σ: GRA.t} (ms: list mname):
+Lemma self_sim_itree `{Σ: GRA.t} `{ns: gnames} (ms: list mname):
   forall n mrs fr st
          (WF: wf_function ms st)
          (MRS: wf_mrs ms mrs),
-    @sim_itree _ (fun p => fst p = snd p /\ wf_mrs ms (fst p))
+    @sim_itree _ (fun p => fst p = snd p /\ wf_mrs ms (fst p)) ns
                n ((mrs, fr), st) ((mrs, fr), st).
 Proof.
   pcofix CIH. i. pfold. punfold WF. inv WF; pclearbot.
@@ -867,6 +892,7 @@ Module ModSemLPair.
 Section SIMMODSEML.
 
   Context `{Σ: GRA.t}.
+  Context `{ns: gnames}.
   Variable (ms_src ms_tgt: ModSemL.t).
 
   Let W: Type := (alist mname (Σ * Any.t)) * (alist mname (Σ * Any.t)).
@@ -881,7 +907,7 @@ Section SIMMODSEML.
 
 End SIMMODSEML.
 
-Lemma self_sim_mod `{Σ: GRA.t} (ms: ModSemL.t) (WF: wf_mod ms):
+Lemma self_sim_mod `{Σ: GRA.t} `{ns: gnames} (ms: ModSemL.t) (WF: wf_mod ms):
   sim ms ms.
 Proof.
   eapply mk with (wf:=fun p => fst p = snd p /\ wf_mrs (List.map fst ms.(ModSemL.initial_mrs)) (fst p)) (le:=top2); ss.
@@ -980,6 +1006,7 @@ Section ADD.
 
 
   Context `{Σ: GRA.t}.
+  Context `{ns: gnames}.
 
   Let W: Type := (alist mname (Σ * Any.t)) * (alist mname (Σ * Any.t)).
 
@@ -1013,46 +1040,9 @@ Section ADD.
     :
       sim_itree wf1 n ms_src ms_tgt.
   Proof.
-    assert (EQV0: forall w, wf0 w -> wf1 w).
-    { i. apply EQV. auto. }
-    assert (EQV1: forall w, wf1 w -> wf0 w).
-    { i. apply EQV. auto. } clear EQV.
-    revert n ms_src ms_tgt SIM. pcofix CIH. i. pfold.
-    punfold SIM. inv SIM; pclearbot.
-    - econs 1; eauto.
-    - econs 2; eauto.
-    - econs 3; eauto. i.
-      clear WF. hexploit K; eauto. i. des. pclearbot. eauto.
-    - econs 4; eauto. i.
-      hexploit K; eauto. i. des. pclearbot. esplits; eauto.
-    - econs 5; eauto. i.
-      hexploit K; eauto. i. des. pclearbot. esplits; eauto.
-    - econs 6; eauto. i.
-      hexploit K; eauto. i. des. pclearbot. esplits; eauto.
-    - econs 7; eauto.
-    - econs 8; eauto.
-    - econs 9; eauto.
-    - econs 10; eauto.
-    - econs 11; eauto.
-    - econs 12; eauto.
-    - econs 13; eauto.
-    - econs 14; eauto. des. pclearbot. esplits; eauto.
-    - econs 15; eauto. i. hexploit K; eauto.
-    - econs 16; eauto.
-    - econs 17; eauto.
-    - econs 18; eauto.
-    - econs 19; eauto.
-    - econs 20; eauto.
-    - econs 21; eauto.
-    - econs 22; eauto.
-    - econs 23; eauto. i. hexploit K; eauto.
-    - econs 24; eauto. des. pclearbot. esplits; eauto.
-    - econs 25; eauto.
-    - econs 26; eauto.
-    - econs 27; eauto.
-    - econs 28; eauto.
-    - econs 29; eauto.
-    - econs 30; eauto.
+    assert(wf0 = wf1).
+    { extensionality x. apply prop_ext; ss. }
+    subst; ss.
   Qed.
 
   Lemma add_sim_itree ms_src0 ms_src1 ms_tgt0 ms_tgt1 (wf0 wf1: W -> Prop)
@@ -1080,24 +1070,24 @@ Section ADD.
         (add_wf ms_src0 ms_src1 ms_tgt0 ms_tgt1 wf0 wf1) n
         (mrs_src, fr_src, st_src) (mrs_tgt, fr_tgt, st_tgt).
   Proof.
-    pcofix CIH. i.
-    pfold. punfold SIM. inv SIM; pclearbot.
+    i. ginit. { eapply cpn6_wcompat; eauto with paco. } revert_until DISJTGT. gcofix CIH. i.
+    gstep. punfold SIM. inv SIM; pclearbot.
     * econs 1; eauto. econs; eauto.
-    * econs 2. right. eapply CIH; eauto.
+    * econs 2. gbase. eapply CIH; eauto.
     * econs 3; eauto.
       { econs; eauto. }
       { i. inv WF1. exploit K; eauto. i. des. pclearbot.
-        exists i1. right. eapply CIH; eauto. }
+        exists i1. gbase. eapply CIH; eauto. }
     * econs 4; eauto.
-      i. hexploit K; eauto. i. des. pclearbot. esplits; eauto.
+      i. hexploit K; eauto. i. des. pclearbot. esplits; eauto with paco.
     * econs 5; eauto.
-      i. hexploit K; eauto. i. des. pclearbot. esplits; eauto.
+      i. hexploit K; eauto. i. des. pclearbot. esplits; eauto with paco.
     * econs 6; eauto.
-      i. hexploit K; eauto. i. des. pclearbot. esplits; eauto.
+      i. hexploit K; eauto. i. des. pclearbot. esplits; eauto with paco.
     * econs 7; eauto.
       { eapply alist_find_filter; eauto. }
       { eapply alist_find_filter; eauto. }
-      { right. eapply CIH; eauto.
+      { gbase. eapply CIH; eauto.
         { repeat erewrite alist_find_add_filter; eauto. }
         { repeat erewrite alist_add_disjoint_filter; eauto.
           { eapply alist_disjoint_find; eauto. }
@@ -1109,7 +1099,7 @@ Section ADD.
     * econs 8; eauto.
       { eapply alist_find_filter; eauto. }
       { eapply alist_find_filter; eauto. }
-      { right. eapply CIH; eauto.
+      { gbase. eapply CIH; eauto.
         { repeat erewrite alist_find_add_filter; eauto. }
         { repeat erewrite alist_add_disjoint_filter; eauto.
           { eapply alist_disjoint_find; eauto. }
@@ -1118,68 +1108,69 @@ Section ADD.
         { eapply alist_add_nodup; eauto. }
         { eapply alist_add_nodup; eauto. }
       }
-    * econs 9; eauto.
-    * econs 10; eauto.
+    * econs 9; eauto with paco.
+    * econs 10; eauto with paco.
       { eapply alist_find_filter; eauto. }
       { eapply alist_find_filter; eauto. }
-    * econs 11; eauto.
+    * econs 11; eauto with paco.
       { eapply alist_find_filter; eauto. }
       { eapply alist_find_filter; eauto. }
-    * econs 12; eauto.
-    * econs 13; eauto.
-    * econs 14; eauto.
-      i. hexploit K; eauto. i. des. pclearbot. esplits; eauto.
+    * econs 12; eauto with paco.
+    * econs 13; eauto with paco.
+    * econs 14; eauto with paco.
+      i. hexploit K; eauto. i. des. pclearbot. esplits; eauto with paco.
     * econs 15; eauto.
-      i. hexploit K; eauto.
-    * econs 16; eauto.
+      i. hexploit K; eauto with paco.
+    * econs 16; eauto with paco.
       { eapply alist_find_filter; eauto. }
-      right. eapply CIH; eauto.
+      gbase. eapply CIH; eauto.
       { repeat erewrite alist_find_add_filter; eauto. }
       { repeat erewrite alist_add_disjoint_filter; eauto.
         { eapply alist_disjoint_find; eauto. }
       }
       { eapply alist_add_nodup; eauto. }
-    * econs 17; eauto.
+    * econs 17; eauto with paco.
       { eapply alist_find_filter; eauto. }
-      right. eapply CIH; eauto.
+      gbase. eapply CIH; eauto.
       { repeat erewrite alist_find_add_filter; eauto. }
       { repeat erewrite alist_add_disjoint_filter; eauto.
         { eapply alist_disjoint_find; eauto. }
       }
       { eapply alist_add_nodup; eauto. }
-    * econs 18; eauto.
-    * econs 19; eauto.
+    * econs 18; eauto with paco.
+    * econs 19; eauto with paco.
       { eapply alist_find_filter; eauto. }
-    * econs 20; eauto.
+    * econs 20; eauto with paco.
       { eapply alist_find_filter; eauto. }
-    * econs 21; eauto.
-    * econs 22; eauto.
+    * econs 21; eauto with paco.
+    * econs 22; eauto with paco.
     * econs 23; eauto.
-      i. hexploit K; eauto.
+      i. hexploit K; eauto with paco.
     * econs 24; eauto.
-      i. hexploit K; eauto. i. des. pclearbot. esplits; eauto.
-    * econs 25; eauto.
+      i. hexploit K; eauto. i. des. pclearbot. esplits; eauto with paco.
+    * econs 25; eauto with paco.
       { eapply alist_find_filter; eauto. }
-      right. eapply CIH; eauto.
+      gbase. eapply CIH; eauto.
       { repeat erewrite alist_find_add_filter; eauto. }
       { repeat erewrite alist_add_disjoint_filter; eauto.
         { eapply alist_disjoint_find; eauto. }
       }
       { eapply alist_add_nodup; eauto. }
-    * econs 26; eauto.
+    * econs 26; eauto with paco.
       { eapply alist_find_filter; eauto. }
-      right. eapply CIH; eauto.
+      gbase. eapply CIH; eauto.
       { repeat erewrite alist_find_add_filter; eauto. }
       { repeat erewrite alist_add_disjoint_filter; eauto.
         { eapply alist_disjoint_find; eauto. }
       }
       { eapply alist_add_nodup; eauto. }
-    * econs 27; eauto.
-    * econs 28; eauto.
+    * econs 27; eauto with paco.
+    * econs 28; eauto with paco.
       { eapply alist_find_filter; eauto. }
-    * econs 29; eauto.
+    * econs 29; eauto with paco.
       { eapply alist_find_filter; eauto. }
-    * econs 30; eauto.
+    * econs 30; eauto with paco.
+    * econs 31; eauto.
   Qed.
 
   Lemma add_modsempair (ms_src0 ms_src1 ms_tgt0 ms_tgt1: ModSemL.t)
@@ -1347,14 +1338,6 @@ Require Import SimGlobal.
 Module ModLPair.
 Section SIMMOD.
    Context `{Σ: GRA.t}.
-   Variable (md_src md_tgt: ModL.t).
-   Inductive sim: Prop := mk {
-     sim_modsem:
-       <<SIM: ModSemLPair.sim (md_src.(ModL.enclose)) (md_tgt.(ModL.enclose))>>;
-     sim_sk: <<SIM: md_src.(ModL.sk) = md_tgt.(ModL.sk)>>;
-     sim_wf:
-       forall sk (INCL: Sk.incl md_src.(ModL.sk) sk) (SKWF: Sk.wf sk) (WF: ModSemL.wf (md_src.(ModL.get_modsem) sk)), <<WF: ModSemL.wf (md_tgt.(ModL.get_modsem) sk)>>;
-   }.
 
    Hint Resolve cpn6_wcompat: paco.
 
@@ -1451,7 +1434,11 @@ Section SIMMOD.
      eapply OrdArith.lt_add_r. eapply OrdArith.lt_from_nat. eauto.
    Qed.
 
+   Context `{ns: gnames}.
+
    Lemma lift_sim ms_src ms_tgt
+         (* (NAMESPACE: forall fn arg (IN: ~ns fn), (ModSemL.prog ms_src) _ (Call fn arg) = triggerUB) *)
+         (NAMESPACE: forall fn (SOME: is_some (alist_find fn (ModSemL.fnsems ms_src))), ns fn)
          (wf: alist string (Σ * Any.t) * alist string (Σ * Any.t) -> Prop)
          (FNS: forall fn : string,
              option_rel (sim_fsem wf)
@@ -1729,8 +1716,30 @@ Section SIMMOD.
        { eapply arith_lt_2 with (n1:=4); auto. }
        gbase. eapply CIH; eauto.
        Unshelve. all: exact O.
+     - erewrite interp_Es_rE with (rst0:=(mrs_src, fr_src :: frs_src)). ss. mgo.
+       econs; eauto.
+       { eapply arith_lt_2 with (n1:=3); auto. }
+       gstep. econs; eauto.
+       { eapply arith_lt_2 with (n1:=2); auto. }
+       gstep. econs; eauto.
+       { eapply arith_lt_2 with (n1:=1); auto. }
+       cbn. unfold unwrapU, triggerUB. des_ifs.
+       { exfalso. eapply FAIL. eapply NAMESPACE. rewrite Heq. ss. }
+       mgo. gstep. econs; ss.
+       { eapply arith_lt_2 with (n1:=0); auto. }
    Qed.
 
+   Variable (md_src md_tgt: ModL.t).
+
+   Inductive sim: Prop := mk {
+     sim_modsem:
+       <<SIM: ModSemLPair.sim (md_src.(ModL.enclose)) (md_tgt.(ModL.enclose))>>;
+     sim_sk: <<SIM: md_src.(ModL.sk) = md_tgt.(ModL.sk)>>;
+     sim_wf:
+       forall sk (INCL: Sk.incl md_src.(ModL.sk) sk) (SKWF: Sk.wf sk) (WF: ModSemL.wf (md_src.(ModL.get_modsem) sk)), <<WF: ModSemL.wf (md_tgt.(ModL.get_modsem) sk)>>;
+   }.
+
+   Hypothesis NAMESPACE: forall fn (SOME: is_some (alist_find fn (ModSemL.fnsems (ModL.get_modsem md_src (Sk.sort (ModL.sk md_src)))))), ns fn.
 
    Theorem adequacy_local_closed
            (SIM: sim)
@@ -1779,6 +1788,7 @@ Section SIMMOD.
      des_ifs_safe. ss. mgo.
      guclo bindC_spec. econs.
      { gfinal. right. eapply lift_sim.
+       { et. }
        { eapply FNS. }
        { eapply x. }
        { ii. unfold ModSemL.initial_p_state. des_ifs. }
